fixing some poly code

code/poly1305/Hacl.Impl.Poly1305_64.fst
@@ -188,8 +188,7 @@ let poly1305_init_ st key =
   log
 
 
-(* #set-options "--z3rlimit 100 --initial_fuel 0 --max_fuel 0 --initial_ifuel 0 --max_ifuel 0" *)
-#set-options "--lax"
+#set-options "--z3rlimit 100 --initial_fuel 0 --max_fuel 0 --initial_ifuel 0 --max_ifuel 0"
 
 val poly1305_update:
   current_log:log_t ->
@@ -229,7 +228,7 @@ let poly1305_update log st m =
   let h5 = ST.get() in
   let m' = elift2_p #wordB_16 #HyperStack.mem #(fun m h -> live h m) #Spec.word
                     (fun m h -> as_seq h m) (hide m) (hide h0) in
-  elift2 (fun l m -> FStar.Seq.(l @| (Seq.create 1 m))) log m'
+  elift2 (fun l m -> FStar.Seq.((Seq.create 1 m) @| l)) log m'
 
 
 #reset-options "--initial_fuel 0 --max_fuel 0 --initial_ifuel 0 --max_ifuel 0 --z3rlimit 100"
@@ -281,7 +280,6 @@ val poly1305_process_last_block_:
       /\ Spec.MkState (as_seq h1 st.r) (as_seq h1 st.h) (reveal updated_log) == Hacl.Spec.Poly1305_64.poly1305_process_last_block_spec (Spec.MkState (as_seq h0 st.r) (as_seq h0 st.h) (reveal current_log)) (as_seq h0 m) (len)
     ))
 [@"c_inline"]
-#set-options "--lax"
 let poly1305_process_last_block_ log block st m rem' =
   let h0 = ST.get() in
   push_frame();
@@ -297,7 +295,7 @@ let poly1305_process_last_block_ log block st m rem' =
   pop_frame();
   let m' = elift2_p #wordB #HyperStack.mem #(fun m h -> live h m) #Spec.word
                     (fun m h -> as_seq h m) (hide m) (hide h0) in
-  elift2 (fun l m -> FStar.Seq.(l @| (Seq.create 1 m))) log m'
+  elift2 (fun l m -> FStar.Seq.((Seq.create 1 m) @| l)) log m'
   
 
 #reset-options "--initial_fuel 0 --max_fuel 0 --initial_ifuel 0 --max_ifuel 0 --z3rlimit 20"
@@ -386,6 +384,8 @@ let carry_limb_unrolled acc =
   upd_3 acc a0' a1' a2'
 
 
+#reset-options "--z3rlimit 100 --initial_fuel 0 --max_fuel 0 --initial_ifuel 0 --max_ifuel 0"
+
 val carry_last_unrolled:
   acc:felem ->
   Stack unit
@@ -396,7 +396,6 @@ val carry_last_unrolled:
       /\ live h1 acc /\ bounds (as_seq h1 acc) p44 p44 p42
       /\ modifies_1 acc h0 h1
       /\ as_seq h1 acc == Hacl.Spec.Poly1305_64.carry_last_unrolled (as_seq h0 acc)))
-#set-options "--lax"
 let carry_last_unrolled acc =
   let h = ST.get() in
   lemma_carried_is_fine_to_carry_top (as_seq h acc);
@@ -484,24 +483,6 @@ inline_for_extraction let poly1305_finish__ log st mac m len key_s =
 
 #reset-options "--initial_fuel 0 --max_fuel 0 --z3rlimit 100"
 
-(* val poly1305_finish_spec: *)
-(*   st:Spec.poly1305_state_{red_44 Spec.(MkState?.r st) /\ red_45 Spec.(MkState?.h st)} -> *)
-(*   m:word -> *)
-(*   rem':limb{v rem' = Seq.length m /\ Seq.length m < 16} -> *)
-(*   key_s:Seq.seq H8.t{Seq.length key_s = 16} -> *)
-(*   Tot word_16 *)
-(* let poly1305_finish_spec st m rem' key_s = *)
-(*   let st' = if U64.(rem' =^ 0uL) then st *)
-(*            else poly1305_process_last_block_spec st m rem' in *)
-(*   let acc = poly1305_last_pass_spec Spec.(MkState?.h st') in *)
-(*   let k' = load128_le_spec key_s in *)
-(*   let open Hacl.Bignum.Wide in *)
-(*   let acc' = Spec.bignum_to_128 acc in *)
-(*   let mac = acc' +%^ k' in *)
-(*   let mac = store128_le_spec mac in *)
-(*   mac *)
-
-
 val poly1305_finish_:
   log:log_t ->
   st:poly1305_state ->
@@ -537,7 +518,10 @@ let poly1305_finish_ log st mac m len key_s =
   let open Hacl.Bignum.Wide in
   let acc' = bignum_to_128 acc in
   let mac' = acc' +%^ k' in
-  hstore128_le mac mac'
+  hstore128_le mac mac';
+  let h1 = ST.get() in
+  lemma_little_endian_inj (Hacl.Spec.Endianness.reveal_sbytes (as_seq h1 mac)) (Hacl.Spec.Poly1305_64.poly1305_finish_spec (Spec.MkState (as_seq h0 st.r) (as_seq h0 st.h) (reveal log)) (as_seq h0 m) len (as_seq h0 key_s))
+
 
 
 (* ************************************************ *)
